backend/CSEproof_linker.v
@@ -83,7 +83,7 @@ Inductive match_call: state -> state -> Prop :=
   | match_states_call:
       forall s f tf args m s' args' m',
       match_stackframes s s' ->
-      globfun_weak_lsim Language_RTL Language_RTL transf_sigT ge tge f tf ->
+      globfun_weak_lsim Language_RTL Language_RTL transf_sigT transf_efT ge tge f tf ->
       Val.lessdef_list args args' ->
       Mem.extends m m' ->
       match_call (Callstate s f args m)
@@ -442,7 +442,7 @@ Hypothesis (Hftprog: program_linkeq Language_RTL tprog ftprog).
 
 Lemma match_states_state_lsim es es' eF F i s1 s1'
       (MS: match_states_ext fprog ftprog s1 s1'):
-  @state_lsim Language_ext_RTL Language_ext_RTL transf_sigT _
+  @state_lsim Language_ext_RTL Language_ext_RTL transf_sigT transf_efT _
               mrelT_ops fprog ftprog es es' eF F i s1 s1'.
 Proof.
   revert F i s1 s1' MS. pcofix CIH. intros F i s1 s1' MS. pfold.
@@ -477,7 +477,7 @@ Qed.
 Lemma transf_function'_lsim
       f approx
       (ANALYZE: analyze f (vanalyze (romem_for_program prog) f) = Some approx):
-  @function_lsim Language_ext_RTL Language_ext_RTL transf_sigT _
+  @function_lsim Language_ext_RTL Language_ext_RTL transf_sigT transf_efT _
                  mrelT_ops fprog ftprog f (transf_function' f approx).
 Proof.
   constructor. intros. pfold. constructor; subst; auto.
@@ -517,7 +517,7 @@ End STATE_LSIM.
 
 Lemma CSE_program_lsim:
   @program_lsim Language_RTL Language_RTL transf_sigT transf_efT transf_vT
-                (@function_lsim Language_ext_RTL Language_ext_RTL transf_sigT _ mrelT_ops)
+                (@function_lsim Language_ext_RTL Language_ext_RTL transf_sigT transf_efT _ mrelT_ops)
                 prog tprog.
 Proof.
   generalize transf_function'_lsim.
