backend/Deadcodeproof_linker.v
@@ -70,7 +70,7 @@ Lemma find_function_translated:
   find_function ge ros rs = Some fd ->
   eagree rs trs (add_ros_need_all ros ne) ->
   exists tfd, find_function tge ros trs = Some tfd /\
-              globfun_weak_lsim Language_RTL Language_RTL transf_sigT ge tge fd tfd.
+              globfun_weak_lsim Language_RTL Language_RTL transf_sigT transf_efT ge tge fd tfd.
 Proof.
   intros. destruct ros as [r|id]; simpl in *.
 - assert (LD: Val.lessdef rs#r trs#r) by eauto with na. inv LD.
@@ -116,7 +116,7 @@ Inductive match_call: state -> state -> Prop :=
   | match_call_states:
       forall s f args m ts tf targs tm
         (STACKS: list_forall2 match_stackframes s ts)
-        (FUN: globfun_weak_lsim Language_RTL Language_RTL transf_sigT ge tge f tf)
+        (FUN: globfun_weak_lsim Language_RTL Language_RTL transf_sigT transf_efT ge tge f tf)
         (ARGS: Val.lessdef_list args targs)
         (MEM: Mem.extends m tm),
       match_call (Callstate s f args m)
@@ -635,7 +635,7 @@ Hypothesis (Hftprog: program_linkeq Language_RTL tprog ftprog).
 
 Lemma match_states_state_lsim es es' eF F i s1 s1'
       (MS: match_states_ext fprog ftprog s1 s1'):
-  @state_lsim Language_ext_RTL Language_ext_RTL transf_sigT _
+  @state_lsim Language_ext_RTL Language_ext_RTL transf_sigT transf_efT _
               mrelT_ops fprog ftprog es es' eF F i s1 s1'.
 Proof.
   revert F i s1 s1' MS. pcofix CIH. intros F i s1 s1' MS. pfold.
@@ -669,7 +669,7 @@ Qed.
 
 Lemma transf_function_lsim
       f tf (Hf: transf_function (romem_for_program prog) f = OK tf):
-  @function_lsim Language_ext_RTL Language_ext_RTL transf_sigT _
+  @function_lsim Language_ext_RTL Language_ext_RTL transf_sigT transf_efT _
                  mrelT_ops fprog ftprog f tf.
 Proof.
   constructor. intros. pfold. constructor; subst; auto.
@@ -718,7 +718,7 @@ End STATE_LSIM.
 
 Lemma Deadcode_program_lsim:
   @program_lsim Language_RTL Language_RTL transf_sigT transf_efT transf_vT
-                (@function_lsim Language_ext_RTL Language_ext_RTL transf_sigT _ mrelT_ops)
+                (@function_lsim Language_ext_RTL Language_ext_RTL transf_sigT transf_efT _ mrelT_ops)
                 prog tprog.
 Proof.
   generalize transf_function_lsim.
