backend/Tailcallproof_linker.v
@@ -90,7 +90,7 @@ Inductive match_call: state -> state -> Prop :=
   | match_states_call:
       forall s f args m s' f' args' m',
       match_stackframes s s' ->
-      globfun_weak_lsim Language_RTL Language_RTL transf_sigT ge tge f f' ->
+      globfun_weak_lsim Language_RTL Language_RTL transf_sigT transf_efT ge tge f f' ->
       Val.lessdef_list args args' ->
       Mem.extends m m' ->
       match_call (Callstate s f args m)
@@ -385,7 +385,7 @@ Hypothesis (Hftprog: program_linkeq Language_RTL tprog ftprog).
 
 Lemma match_states_state_lsim es es' eF F s1 s1'
       (MS: match_states_ext fprog ftprog s1 s1'):
-  @state_lsim Language_ext_RTL Language_ext_RTL transf_sigT _
+  @state_lsim Language_ext_RTL Language_ext_RTL transf_sigT transf_efT _
               mrelT_ops fprog ftprog es es' eF F (WF.from_nat (measure s1)) s1 s1'.
 Proof.
   revert F s1 s1' MS. pcofix CIH. intros F s1 s1' MS. pfold.
@@ -435,7 +435,7 @@ Proof.
 Qed.
 
 Lemma transf_function_lsim f:
-  @function_lsim Language_ext_RTL Language_ext_RTL transf_sigT _
+  @function_lsim Language_ext_RTL Language_ext_RTL transf_sigT transf_efT _
                  mrelT_ops fprog ftprog f (transf_function f).
 Proof.
   constructor. intros. pfold. constructor; subst; auto.
@@ -477,7 +477,7 @@ End STATE_LSIM.
 
 Lemma Tailcall_program_lsim:
   @program_lsim Language_RTL Language_RTL transf_sigT transf_efT transf_vT
-                (@function_lsim Language_ext_RTL Language_ext_RTL transf_sigT _ mrelT_ops)
+                (@function_lsim Language_ext_RTL Language_ext_RTL transf_sigT transf_efT _ mrelT_ops)
                 prog tprog.
 Proof.
   generalize transf_function_lsim.
